pure pre/post on selector return value

examples/steel/Selectors.Loops.fst
@@ -16,10 +16,8 @@ let rec fact
 
 (* Steel implementation *)
 
-let fact_test_vpre_refine
+let fact_test_pre
   (n: nat)
-  (i: ref nat)
-  (res: ref nat)
   (dist: Ghost.erased nat)
   (x: (nat & nat))
 : Tot prop
@@ -27,68 +25,48 @@ let fact_test_vpre_refine
   let vres = snd x in
   vres == fact vi /\ vi + Ghost.reveal dist == n
 
-let fact_test_vpre
-  (n: nat)
+[@@ __steel_reduce__ ] // necessary for t_of
+let fact_test_vprop
   (i: ref nat)
   (res: ref nat)
   (dist: Ghost.erased nat)
 : Tot vprop
-= (vptr i `star` vptr res) `vrefine` (fact_test_vpre_refine n i res dist)
+= (vptr i `star` vptr res)
 
-let fact_test_vpost_refine
-  (dist: Ghost.erased nat)
+let fact_test_post
+  (n: nat)
   (b: bool)
-  (_: t_of emp)
+  (dist: Ghost.erased nat)
+  (x: (nat & nat))
 : Tot prop
-= b == (Ghost.reveal dist > 0)
-
-let fact_test_vpost
-  (n: nat)
-  (i: ref nat)
-  (res: ref nat)
-  (b: bool)
-  (dist: Ghost.erased nat)
-: Tot vprop
-= fact_test_vpre n i res dist `star` (emp `vrefine` fact_test_vpost_refine dist b)
+= fact_test_pre n dist x /\
+  b == (Ghost.reveal dist > 0)
 
 let fact_test
   (n: nat)
   (i: ref nat)
   (res: ref nat)
   (dist: Ghost.erased nat)
-: SteelSelT bool
-    (fact_test_vpre n i res dist)
-    (fun b -> fact_test_vpost n i res b dist)
-= change_equal_slprop
-    (fact_test_vpre n i res dist)
-    ((vptr i `star` vptr res) `vrefine` fact_test_vpre_refine n i res dist);
-  elim_vrefine
-    (vptr i `star` vptr res)
-    (fact_test_vpre_refine n i res dist);
+: SteelSel bool
+    (fact_test_vprop i res dist)
+    (fun b -> fact_test_vprop i res dist)
+    (fun h -> fact_test_pre n dist (h (fact_test_vprop i res dist)))
+    (fun _ b h' -> fact_test_post n b dist (h' (fact_test_vprop i res dist)))
+=
+  change_equal_slprop
+    (fact_test_vprop i res dist)
+    (vptr i `star` vptr res);
   reveal_star (vptr i) (vptr res);
+  let gres = gget (vptr res) in
   let vi = read i in
+  assert (Ghost.reveal gres == fact vi);
+  assert (vi + Ghost.reveal dist == n);
   let b = (vi < n) in
   reveal_star (vptr i) (vptr res);
-  intro_vrefine
-    (vptr i `star` vptr res)
-    (fact_test_vpre_refine n i res dist);
-  intro_vrefine
-    emp
-    (fact_test_vpost_refine dist b);
-  assert_norm (
-    ((vptr i `star` vptr res) `vrefine` fact_test_vpre_refine n i res dist) `star` (emp `vrefine` fact_test_vpost_refine dist b) ==
-    fact_test_vpost n i res b dist
-  );
   change_equal_slprop
-    (((vptr i `star` vptr res) `vrefine` fact_test_vpre_refine n i res dist) `star` (emp `vrefine` fact_test_vpost_refine dist b))
-    (fact_test_vpost n i res b dist);
+    (vptr i `star` vptr res)
+    (fact_test_vprop i res dist);
   return b
-
-let change_equal_slprop_with_squash (#opened:_) (p q: vprop)
-  (sq: squash (p == q))
-  : SteelSelGhost unit opened p (fun _ -> q) (fun _ -> True) (fun h0 _ h1 -> p == q /\ h1 q == h0 p)
-=
-  change_equal_slprop p q
 
 let fact_body
   (n: nat)
@@ -96,44 +74,29 @@ let fact_body
   (res: ref nat)
   (dist: Ghost.erased nat)
 : SteelSel (Ghost.erased nat)
-    (fact_test_vpost n i res true dist)
-    (fun dist -> fact_test_vpre n i res dist)
-    (fun _ -> True)
-    (fun _ dist' _ -> Ghost.reveal dist' << Ghost.reveal dist)
+    (fact_test_vprop i res dist)
+    (fun dist -> fact_test_vprop i res dist)
+    (fun h -> fact_test_post n true dist (h (fact_test_vprop i res dist)))
+    (fun _ dist' h' -> fact_test_pre n dist' (h' (fact_test_vprop i res dist')) /\ Ghost.reveal dist' << Ghost.reveal dist)
 =
-  let sq : squash (
-    ((vptr i `star` vptr res) `vrefine` fact_test_vpre_refine n i res dist) `star` (emp `vrefine` fact_test_vpost_refine dist true) ==
-    fact_test_vpost n i res true dist
-  ) = () in
-  change_equal_slprop_with_squash
-    (fact_test_vpost n i res true dist)
-    (((vptr i `star` vptr res) `vrefine` fact_test_vpre_refine n i res dist) `star` (emp `vrefine` fact_test_vpost_refine dist true))
-    sq;
-  elim_vrefine
-    emp
-    (fact_test_vpost_refine dist true);
-  elim_vrefine
-    (vptr i `star` vptr res)
-    (fact_test_vpre_refine n i res dist);
+  change_equal_slprop
+    (fact_test_vprop i res dist)
+    (vptr i `star` vptr res);
   reveal_star (vptr i) (vptr res);
   let vi = read i in
   let vj = vi + 1 in
   let vres = read res in
   write res (vj * vres);
   write i vj;
-  reveal_star (vptr i) (vptr res);
   let dist' = Ghost.hide (Ghost.reveal dist - 1) in
-  intro_vrefine
+  let gres = gget (vptr res) in
+  let gi = gget (vptr i) in
+  assert (Ghost.reveal gres == fact (Ghost.reveal gi));
+  assert (Ghost.reveal gi + Ghost.reveal dist' == n);
+  reveal_star (vptr i) (vptr res);
+  change_equal_slprop
     (vptr i `star` vptr res)
-    (fact_test_vpre_refine n i res dist');
-  let sq : squash (
-    ((vptr i `star` vptr res) `vrefine` fact_test_vpre_refine n i res dist')
-      == fact_test_vpre n i res dist'
-  ) = _ by (FStar.Tactics.trefl ()) in
-  change_equal_slprop_with_squash
-    ((vptr i `star` vptr res) `vrefine` fact_test_vpre_refine n i res dist')
-    (fact_test_vpre n i res dist')
-    ();
+    (fact_test_vprop i res dist');
   return dist'
 
 (* this is necessary, otherwise verification of steel_fact fails to show fact_test_pre *)
@@ -156,28 +119,13 @@ let steel_fact
   let res = alloc 1 in
   let dist = Ghost.hide n in
   reveal_star (vptr i) (vptr res);
-  intro_vrefine
-    (vptr i `star` vptr res)
-    (fact_test_vpre_refine n i res dist);
-  assert_norm
-    ((vptr i `star` vptr res) `vrefine` fact_test_vpre_refine n i res dist ==
-    fact_test_vpre n i res dist);
   change_equal_slprop
-    ((vptr i `star` vptr res) `vrefine` fact_test_vpre_refine n i res dist)
-    (fact_test_vpre n i res dist);
-  let dist' = while _ (fact_test_vpre n i res) (fact_test_vpost n i res) (fact_test n i res) (fact_body n i res) dist in
-  assert_norm
-    (fact_test_vpost n i res false dist' ==
-    ((vptr i `star` vptr res) `vrefine` fact_test_vpre_refine n i res dist') `star` (emp `vrefine` fact_test_vpost_refine dist' false));
-  change_equal_slprop
-    (fact_test_vpost n i res false dist')
-    (((vptr i `star` vptr res) `vrefine` fact_test_vpre_refine n i res dist') `star` (emp `vrefine` fact_test_vpost_refine dist' false));
-  elim_vrefine
-    emp
-    (fact_test_vpost_refine dist' false);
-  elim_vrefine
     (vptr i `star` vptr res)
-    (fact_test_vpre_refine n i res dist');
+    (fact_test_vprop i res dist);
+  let dist' = while _ (fact_test_vprop i res) (fact_test_pre n) (fun _ -> fact_test_vprop i res) (fact_test_post n) (fact_test n i res) (fact_body n i res) dist in
+  change_equal_slprop
+    (fact_test_vprop i res dist')
+    (vptr i `star` vptr res);
   reveal_star (vptr i) (vptr res);
   let gi = gget (vptr i) in // necessary to tell Z3 to show that i == n
   let vres = read res in
