ulib/experimental/Steel.SelLoops.fst
@@ -4,11 +4,12 @@ open Steel.SelEffect
 open Steel.SelEffect.Atomic
 
 let rec while
-  t test_vpre test_vpost test body x0
-: SteelSelT
-  (Ghost.erased t)
+  t test_vpre test_pre test_vpost test_post test body x0
+: SteelSel (Ghost.erased t)
     (test_vpre x0)
     (fun res -> test_vpost false res)
+    (fun h -> test_pre x0 (h (test_vpre x0)))
+    (fun _ res h' -> test_post false res (h' (test_vpost false res)))
   (decreases (Ghost.reveal x0))
 =
   let b = test x0 in
@@ -18,7 +19,7 @@ let rec while
       (test_vpost b x0)
       (test_vpost true x0);
     let x1 = body x0 in
-    while t test_vpre test_vpost test body x1
+    while t test_vpre test_pre test_vpost test_post test body x1
   end else begin
     change_equal_slprop
       (test_vpost b x0)
