ulib/experimental/Steel.SelLoops.fsti
@@ -7,21 +7,28 @@ open Steel.SelEffect
 val while
   (t: Type)
   (test_vpre: (Ghost.erased t -> vprop))
+  (test_pre: (x: Ghost.erased t) -> (y: (t_of (test_vpre x))) -> Tot prop)
   (test_vpost: bool -> Ghost.erased t -> Tot vprop)
+  (test_post: (b: bool) -> (x: Ghost.erased t) -> (y: (t_of (test_vpost b x))) -> Tot prop)
   (test: (e: Ghost.erased t) ->
-    SteelSelT bool
+    SteelSel bool
     (test_vpre e)
     (fun x -> test_vpost x e)
+    (fun h -> test_pre e (h (test_vpre e)))
+    (fun _ b h' -> test_post b e (h' (test_vpost b e)))
   )
   (body: (e: Ghost.erased t) -> SteelSel (Ghost.erased t)
     (test_vpost true e)
     (fun res -> test_vpre res)
-    (fun _ -> True)
-    (fun _ res _ ->
+    (fun h -> test_post true e (h (test_vpost true e)))
+    (fun _ res h' ->
+      test_pre res (h' (test_vpre res)) /\
       Ghost.reveal res << Ghost.reveal e
     )
   )
   (x0: Ghost.erased t)
-: SteelSelT (Ghost.erased t)
+: SteelSel (Ghost.erased t)
     (test_vpre x0)
     (fun res -> test_vpost false res)
+    (fun h -> test_pre x0 (h (test_vpre x0)))
+    (fun _ res h' -> test_post false res (h' (test_vpost false res)))
